Tests.lean
@@ -1,5 +1,5 @@
 import Tests.matmul
---import Tests.fori_loop
+import Tests.fori_loop
 --import Tests.index_nonzero
 import Tests.scatter
 --import Tests.normalize
